Splinter/BranchTreeInterp.i.dfy
@@ -7,7 +7,7 @@ include "BranchTree.i.dfy"
 include "SplinterTree.i.dfy"
 include "../Spec/Message.s.dfy"
 include "../Spec/Interp.s.dfy"
-
+include "../lib/Base/mathematics.i.dfy"
 
 module BranchTreeInterpMod {
   import opened Options
@@ -21,6 +21,7 @@ module BranchTreeInterpMod {
   import opened BranchTreeMod
   import SplinterTreeMachineMod
   import Nat_Order
+  import opened Mathematics
 
   type Lookup = BranchPath
 
@@ -48,5 +49,46 @@ module BranchTreeInterpMod {
   }
 
   function IReadsKey(v: Variables, cache: CacheIfc.Variables, key: Key) : set<CU>
+
+  function IReads(v: Variables, cache: CacheIfc.Variables) : set<CU>
+
+  lemma BranchLookupsEquivalentInductive(v: Variables,
+                                cache0: CacheIfc.Variables,
+                                cache1: CacheIfc.Variables,
+                                lookup0: BranchPath,
+                                lookup1: BranchPath,
+                                count : nat)
+    requires lookup0.key == lookup1.key
+    requires lookup0.Valid(cache0)
+    requires lookup1.Valid(cache1)
+    requires count <= |lookup0.steps|
+    requires count <= |lookup1.steps|
+    requires DiskViewsEquivalent(cache0.dv, cache1.dv, IReads(v, cache0))
+    ensures forall i :: ((0 <= i < count) ==> (lookup0.steps[i] == lookup1.steps[i]))
+    {
+      if count == 0 {
+
+      } else {
+        BranchLookupsEquivalentInductive(v, cache0, cache1, lookup0, lookup1, count - 1);
+        var step0 :=  lookup0.steps[count-1];
+        var step1 :=  lookup1.steps[count-1];
+      }
+    }
+
+
+    lemma BranchLookupsEquivalent(v: Variables,
+                                  cache0: CacheIfc.Variables,
+                                  cache1: CacheIfc.Variables,
+                                  lookup0: BranchPath,
+                                  lookup1: BranchPath)
+      requires lookup0.key == lookup1.key
+      requires lookup0.Valid(cache0)
+      requires lookup1.Valid(cache1)
+      requires DiskViewsEquivalent(cache0.dv, cache1.dv, IReads(v, cache0))
+      ensures  lookup0 == lookup1
+      {
+        var minLookup := min(|lookup0.steps|, |lookup1.steps|);
+        BranchLookupsEquivalentInductive(v, cache0, cache1, lookup0, lookup1, minLookup);
+      }
 
 }
